IDA/EDA soudness

DegreeofAmbiguity.v
@@ -1,7 +1,7 @@
-Require Import List Arith Lia.
+From Stdlib Require Import List Arith Bool Lia.
 Import ListNotations.
 
-From PositionAutomata Require Import PositionAutomaton.
+From PositionAutomata Require Import Sets Syntax PositionAutomaton.
 
 (** Basic definitions for the degree of ambiguity of finite automata.
 
@@ -44,6 +44,31 @@ Proof.
     lia.
 Qed.
 
+Lemma sum_nats_pos_In :
+  forall xs,
+    0 < sum_nats xs ->
+    exists x, In x xs /\ 0 < x.
+Proof.
+  induction xs as [| x xs IH]; simpl; intros Hpos.
+  - lia.
+  - destruct x as [| x'].
+    + destruct (IH Hpos) as [y [Hy Hlt]].
+      exists y. split; simpl; auto.
+    + exists (S x'). split; simpl; auto; lia.
+Qed.
+
+Lemma sum_map_pos_In :
+  forall {B : Type} (f : B -> nat) xs,
+    0 < sum_nats (map f xs) ->
+    exists x, In x xs /\ 0 < f x.
+Proof.
+  intros B f xs Hpos.
+  apply sum_nats_pos_In in Hpos as [n [Hin Hn]].
+  apply in_map_iff in Hin as [x [Hx Hin]].
+  subst.
+  exists x. split; assumption.
+Qed.
+
 Section NFA.
   Context {A : Type}.
 
@@ -53,6 +78,48 @@ Section NFA.
     nfa_final : nfa_state -> bool;
     nfa_step : nfa_state -> A -> list nfa_state
   }.
+
+  Record finite_nfa : Type := {
+    fnfa_base :> nfa;
+    fnfa_states : list (nfa_state fnfa_base);
+    fnfa_alphabet : list A;
+    fnfa_state_eqb : nfa_state fnfa_base -> nfa_state fnfa_base -> bool;
+    fnfa_state_eqb_sound :
+      forall x y, fnfa_state_eqb x y = true -> x = y;
+    fnfa_state_eqb_complete :
+      forall x y, x = y -> fnfa_state_eqb x y = true
+  }.
+
+  Inductive path_from (m : nfa)
+      : nfa_state m -> list A -> nfa_state m -> Prop :=
+  | Path_nil :
+      forall q,
+        path_from m q [] q
+  | Path_cons :
+      forall q a q' w q'',
+        In q' (nfa_step m q a) ->
+        path_from m q' w q'' ->
+        path_from m q (a :: w) q''.
+
+  Definition delta_star (m : nfa) : nfa_state m -> list A -> nfa_state m -> Prop :=
+    path_from m.
+
+  Definition accepting_path (m : nfa) (w : list A) : Prop :=
+    exists q0 qf,
+      In q0 (nfa_start m) /\
+      path_from m q0 w qf /\
+      nfa_final m qf = true.
+
+  Definition useful_state (m : nfa) (q : nfa_state m) : Prop :=
+    exists q0 qf w1 w2,
+      In q0 (nfa_start m) /\
+      path_from m q0 w1 q /\
+      path_from m q w2 qf /\
+      nfa_final m qf = true.
+
+  Definition connected (m : nfa) (p q : nfa_state m) : Prop :=
+    exists u v,
+      path_from m p u q /\ path_from m q v p.
 
   Fixpoint accepting_runs_from
       (m : nfa)
@@ -66,6 +133,9 @@ Section NFA.
 
   Definition ambiguity_of_word (m : nfa) (w : list A) : nat :=
     sum_nats (map (fun q => accepting_runs_from m q w) (nfa_start m)).
+
+  Definition infinitely_ambiguous (m : nfa) : Prop :=
+    forall k, exists w, k <= ambiguity_of_word m w.
 
   Fixpoint words_of_length (alphabet : list A) (n : nat) : list (list A) :=
     match n with
@@ -100,6 +170,174 @@ Section NFA.
     exists c b,
       2 <= b /\
       forall w, ambiguity_of_word m w <= c * Nat.pow b (length w).
+
+  Fixpoint runs_between
+      (m : finite_nfa)
+      (q : nfa_state (fnfa_base m))
+      (w : list A)
+      (r : nfa_state (fnfa_base m)) : nat :=
+    match w with
+    | [] => if fnfa_state_eqb m q r then 1 else 0
+    | a :: w' =>
+        sum_nats
+          (map
+             (fun q' => runs_between m q' w' r)
+             (nfa_step (fnfa_base m) q a))
+    end.
+
+  Definition da_from_to := runs_between.
+
+  Definition start_runs_to
+      (m : finite_nfa)
+      (w : list A)
+      (q : nfa_state (fnfa_base m)) : nat :=
+    sum_nats
+      (map
+         (fun q0 => runs_between m q0 w q)
+         (nfa_start (fnfa_base m))).
+
+  Lemma runs_between_positive_path :
+    forall (m : finite_nfa) q w r,
+      0 < runs_between m q w r ->
+      path_from (fnfa_base m) q w r.
+  Proof.
+    intros m q w.
+    generalize dependent q.
+    induction w as [| a w IH]; intros q r Hpos; simpl in Hpos.
+    - destruct (fnfa_state_eqb m q r) eqn:Heq; try lia.
+      apply fnfa_state_eqb_sound in Heq. subst.
+      constructor.
+    - apply sum_map_pos_In in Hpos as [q' [Hin Hpos]].
+      eapply Path_cons; eauto.
+  Qed.
+
+  Lemma start_runs_to_positive_path :
+    forall (m : finite_nfa) w q,
+      0 < start_runs_to m w q ->
+      exists q0,
+        In q0 (nfa_start (fnfa_base m)) /\
+        path_from (fnfa_base m) q0 w q.
+  Proof.
+    intros m w q Hpos.
+    unfold start_runs_to in Hpos.
+    apply sum_map_pos_In in Hpos as [q0 [Hin Hpos]].
+    exists q0. split; auto.
+    now apply runs_between_positive_path.
+  Qed.
+
+  Lemma accepting_runs_from_positive_path :
+    forall (m : nfa) q w,
+      0 < accepting_runs_from m q w ->
+      exists qf,
+        path_from m q w qf /\
+        nfa_final m qf = true.
+  Proof.
+    intros m q w.
+    revert q.
+    induction w as [| a w IH]; intros q Hpos; simpl in Hpos.
+    - destruct (nfa_final m q) eqn:Hfinal; try lia.
+      exists q. split; constructor || assumption.
+    - apply sum_map_pos_In in Hpos as [q' [Hin Hpos]].
+      destruct (IH q' Hpos) as [qf [Hpath Hfinal]].
+      exists qf. split; auto.
+      eapply Path_cons; eauto.
+  Qed.
+
+  Lemma useful_state_from_positive_tests :
+    forall (m : finite_nfa) q w_in w_out,
+      0 < start_runs_to m w_in q ->
+      0 < accepting_runs_from (fnfa_base m) q w_out ->
+      useful_state (fnfa_base m) q.
+  Proof.
+    intros m q w_in w_out Hin Hout.
+    destruct (start_runs_to_positive_path m w_in q Hin) as [q0 [Hstart Hpath_in]].
+    destruct (accepting_runs_from_positive_path (fnfa_base m) q w_out Hout)
+      as [qf [Hpath_out Hfinal]].
+    unfold useful_state.
+    exists q0, qf, w_in, w_out.
+    repeat split; assumption.
+  Qed.
+
+  Definition option_nat_eqb (x y : option nat) : bool :=
+    match x, y with
+    | None, None => true
+    | Some x', Some y' => Nat.eqb x' y'
+    | _, _ => false
+    end.
+
+  Lemma option_nat_eqb_sound :
+    forall x y, option_nat_eqb x y = true -> x = y.
+  Proof.
+    intros [x|] [y|]; simpl; intros H; try discriminate; auto.
+    apply Nat.eqb_eq in H. subst. reflexivity.
+  Qed.
+
+  Lemma option_nat_eqb_complete :
+    forall x y, x = y -> option_nat_eqb x y = true.
+  Proof.
+    intros x y H. subst.
+    destruct y as [y|]; simpl; auto.
+    apply Nat.eqb_refl.
+  Qed.
+
+  Definition position_nfa_state : Type := option nat.
+
+  Definition matching_positions
+      (label_matches : A -> A -> bool)
+      (lbl : symbol_at)
+      (ps : list nat)
+      (a : A) : list position_nfa_state :=
+    fold_right
+      (fun p acc =>
+         match lbl p with
+         | Some b =>
+             if label_matches b a then Some p :: acc else acc
+         | None => acc
+         end)
+      []
+      ps.
+
+  Definition position_nfa_step
+      (label_matches : A -> A -> bool)
+      (r : positioned_regex A)
+      (s : position_nfa_state)
+      (a : A) : list position_nfa_state :=
+    let lbl := label_of r in
+    match s with
+    | None => matching_positions label_matches lbl (firstpos r) a
+    | Some p => matching_positions label_matches lbl (lookup_follow p (followpos r)) a
+    end.
+
+  Definition position_nfa_final
+      (r : positioned_regex A)
+      (s : position_nfa_state) : bool :=
+    match s with
+    | None => nullable r
+    | Some p => mem p (lastpos r)
+    end.
+
+  Definition position_nfa
+      (label_matches : A -> A -> bool)
+      (r : positioned_regex A) : nfa :=
+    {|
+      nfa_state := position_nfa_state;
+      nfa_start := [None];
+      nfa_final := position_nfa_final r;
+      nfa_step := position_nfa_step label_matches r
+    |}.
+
+  Definition finite_position_nfa
+      (alphabet : list A)
+      (label_matches : A -> A -> bool)
+      (r : positioned_regex A) : finite_nfa :=
+    {|
+      fnfa_base := position_nfa label_matches r;
+      fnfa_states := None :: map Some (positions r);
+      fnfa_alphabet := alphabet;
+      fnfa_state_eqb := option_nat_eqb;
+      fnfa_state_eqb_sound := option_nat_eqb_sound;
+      fnfa_state_eqb_complete := option_nat_eqb_complete
+    |}.
 
   Definition deterministic_as_nfa (m : @automaton A) : nfa :=
     {|
