Examples.v
@@ -1,7 +1,9 @@
-Require Import List Bool Arith.
+From Stdlib Require Import List Bool Arith.
 Import ListNotations.
 
-From PositionAutomata Require Import Syntax PositionAutomaton Equivalence KleeneSemantics.
+From PositionAutomata Require Import
+  Syntax PositionAutomaton Equivalence KleeneSemantics
+  DegreeofAmbiguity DegreeofInfiniteAmbiguity.
 
 Definition a_then_b : regex bool :=
   Cat (Atom true) (Atom false).
@@ -96,4 +98,118 @@ Example accepts_marked_a_then_b :
 Proof.
   unfold accepts_marked, positioned_a_then_b, a_then_b.
   simpl. repeat split; reflexivity.
+Qed.
+
+Example position_nfa_a_then_b_one_run :
+  ambiguity_of_word
+    (position_nfa Bool.eqb positioned_a_then_b)
+    [true; false] = 1.
+Proof. reflexivity. Qed.
+
+Example position_nfa_a_then_b_no_eda_fuel_2 :
+  edab_with_fuel
+    2
+    (finite_position_nfa [true; false] Bool.eqb positioned_a_then_b) = false.
+Proof. reflexivity. Qed.
+
+Definition ambiguous_a : regex bool :=
+  Alt (Atom true) (Atom true).
+
+Example position_nfa_ambiguous_a_two_runs :
+  ambiguity_of_word
+    (position_nfa Bool.eqb (label ambiguous_a))
+    [true] = 2.
+Proof. reflexivity. Qed.
+
+Definition unit_eqb (_ _ : unit) : bool := true.
+
+Lemma unit_eqb_sound :
+  forall x y, unit_eqb x y = true -> x = y.
+Proof.
+  intros [] [] _. reflexivity.
+Qed.
+
+Lemma unit_eqb_complete :
+  forall x y, x = y -> unit_eqb x y = true.
+Proof.
+  intros [] [] _. reflexivity.
+Qed.
+
+Definition duplicated_loop_nfa : @finite_nfa bool :=
+  {|
+    fnfa_base :=
+      {|
+        nfa_state := unit;
+        nfa_start := [tt];
+        nfa_final := fun _ => true;
+        nfa_step := fun (_ : unit) (a : bool) => if a then [tt; tt] else []
+      |};
+    fnfa_states := [tt];
+    fnfa_alphabet := [true];
+    fnfa_state_eqb := unit_eqb;
+    fnfa_state_eqb_sound := unit_eqb_sound;
+    fnfa_state_eqb_complete := unit_eqb_complete
+  |}.
+
+Example duplicated_loop_word_has_two_runs :
+  ambiguity_of_word duplicated_loop_nfa [true] = 2.
+Proof. reflexivity. Qed.
+
+Example duplicated_loop_edab :
+  edab_with_fuel 1 duplicated_loop_nfa = true.
+Proof. reflexivity. Qed.
+
+Example duplicated_loop_eda :
+  EDA duplicated_loop_nfa.
+Proof.
+  apply edab_with_fuel_sound with (fuel := 1).
+  reflexivity.
+Qed.
+
+Definition nat_state_step (q : nat) (a : bool) : list nat :=
+  if a then
+    match q with
+    | 0 => [0; 1]
+    | 1 => [1]
+    | _ => []
+    end
+  else [].
+
+Lemma nat_eqb_complete :
+  forall x y : nat, x = y -> Nat.eqb x y = true.
+Proof.
+  intros x y H. subst. apply Nat.eqb_refl.
+Qed.
+
+Lemma nat_eqb_sound :
+  forall x y : nat, Nat.eqb x y = true -> x = y.
+Proof.
+  intros x y H. now apply Nat.eqb_eq.
+Qed.
+
+Definition ida_example_nfa : @finite_nfa bool :=
+  {|
+    fnfa_base :=
+      {|
+        nfa_state := nat;
+        nfa_start := [0];
+        nfa_final := fun q => Nat.leb q 1;
+        nfa_step := nat_state_step
+      |};
+    fnfa_states := [0; 1];
+    fnfa_alphabet := [true];
+    fnfa_state_eqb := Nat.eqb;
+    fnfa_state_eqb_sound := nat_eqb_sound;
+    fnfa_state_eqb_complete := nat_eqb_complete
+  |}.
+
+Example ida_example_idab :
+  idab_with_fuel 1 ida_example_nfa = true.
+Proof. reflexivity. Qed.
+
+Example ida_example_satisfies_ida :
+  IDA ida_example_nfa.
+Proof.
+  apply idab_with_fuel_sound with (fuel := 1).
+  reflexivity.
 Qed.
